src/3d/Translate.fst
@@ -284,39 +284,94 @@ let rec translate_expr (e:A.expr) : ML T.expr =
    | This -> failwith "`this` should have been eliminated already"),
   e.A.range
 
+let rec translate_output_type (t:A.typ) : ML T.typ =
+  match t.v with
+  | Pointer t -> T.T_pointer (translate_output_type t)
+  | Type_app id b [] -> T.T_app id b []
+  | _ -> failwith "Impossible, translate_output_type did not get an output type!"
+
+let rec translate_out_expr_node (oe:with_meta_t out_expr')
+  : ML T.output_expr' =
+  match oe.v with
+  | OE_id id -> T.T_OE_id id
+  | OE_star oe -> T.T_OE_star (translate_out_expr oe)
+  | OE_addrof oe -> T.T_OE_addrof (translate_out_expr oe)
+  | OE_deref oe id -> T.T_OE_deref (translate_out_expr oe) id
+  | OE_dot oe id -> T.T_OE_dot (translate_out_expr oe) id
+
+and translate_out_expr (oe:out_expr) : ML T.output_expr =
+  let oe' = translate_out_expr_node oe.out_expr_node in
+  match oe.out_expr_meta with
+  | Some (i, bt, t) ->
+    { T.oe_expr = oe';
+      T.oe_bt = translate_output_type bt;
+      T.oe_t = translate_output_type t;
+      T.oe_base_ident = i }
+  | None -> failwith "Impossible!"
+  
 
 /// An output expression type parameter is translated to a getter
 ///   applied to the base variable
 
-let translate_out_expr_typ_param (oe:out_expr) : ML T.expr =
-  let fn_name = Target.output_getter_name oe in
-  let base_var = Target.output_base_var oe in
-  (T.App (T.Ext fn_name)
-     [(T.Identifier base_var, oe.A.out_expr_node.A.range)]), oe.A.out_expr_node.A.range
+let output_types_attributes = {
+  T.is_hoisted = false;
+  T.is_exported = false;
+  T.should_inline = false;
+  T.comments = [] }
 
-let translate_typ_param (p:typ_param) : ML T.expr =
+let translate_out_expr_typ_param (oe:out_expr) : ML (T.expr & T.decls) =
+  let t_oe = translate_out_expr oe in
+  let fn_name = Target.output_getter_name t_oe in
+  let base_var = Target.output_base_var t_oe in
+  let te =
+    (T.App (T.Ext fn_name)
+      [(T.Identifier base_var, oe.A.out_expr_node.A.range)]), oe.A.out_expr_node.A.range in
+  te, [T.Output_type_expr t_oe true, output_types_attributes]
+  
+  //   Target.Output_type_val oe_bt, output_types_attributes;
+  //   Target.Output_type_val oe_t, output_types_attributes;
+  //   Target.Output_type_getter
+  //     (Printf.sprintf "get_%s" (Target.out_fn_name oe))
+  //     oe_t
+  //     oe_bt
+  //     (Target.ident_name (Target.out_expr_var oe))
+  // let oe_bt, decls1 = translate_typ (A.out_expr_bt oe) in
+  // let oe_t, decls2 = translate_typ (A.out_expr_t oe) in
+  // let decls = [
+  //   Target.Output_type_val oe_bt, output_types_attributes;
+  //   Target.Output_type_val oe_t, output_types_attributes;
+  //   Target.Output_type_getter oe.out_expr_node.v oe_t oe_bt, output_types_attributes] in
+  // te, decls1@decls2@decls
+let translate_typ_param (p:typ_param) : ML (T.expr & T.decls) =
   match p with
-  | A.Inl e  -> translate_expr e
+  | A.Inl e  -> translate_expr e, []
   | A.Inr oe -> translate_out_expr_typ_param oe
 
-let rec translate_typ (t:A.typ) : ML T.typ =
+let rec translate_typ (t:A.typ) : ML (T.typ & T.decls) =
   match t.v with
   | Pointer t ->
-    let t' = translate_typ t in
-    T.T_pointer t'
+    let t', decls = translate_typ t in
+    T.T_pointer t', decls
   | Type_app hd b args ->
-    T.T_app hd b (List.map (fun x -> Inr (translate_typ_param x)) args)
+    let args, decls = List.fold_left (fun (args, decls) arg ->
+      let arg, ds = translate_typ_param arg in
+      args@[arg], decls@ds) ([], []) args in
+    T.T_app hd b (List.map Inr args), decls //(List.map (fun x -> Inr (translate_typ_param x)) args)
 
 let has_entrypoint (l:list A.attribute) =
   List.tryFind (function A.Entrypoint -> true | _ -> false) l
   |> Some?
 
-let translate_typedef_name (tdn:A.typedef_names) (params:list Ast.param) : ML T.typedef_name =
-  let params = List.map (fun (t, id, _) -> id, translate_typ t) params in //TODO: ignoring qualifier
+let translate_typedef_name (tdn:A.typedef_names) (params:list Ast.param)
+  : ML (T.typedef_name & T.decls) =
+  let params, ds =
+    List.fold_left (fun (params, decls) (t, id, _) ->
+      let t, ds = translate_typ t in
+      params@[id, t], decls@ds) ([], []) params in //TODO: ignoring qualifier
   let open T in
   { td_name = tdn.typedef_name;
     td_params = params;
-    td_entrypoint = has_entrypoint tdn.typedef_attributes }
+    td_entrypoint = has_entrypoint tdn.typedef_attributes }, ds
 
 let make_enum_typ (t:T.typ) (ids:list ident) =
   let refinement i =
@@ -517,54 +572,76 @@ let make_reader (env:global_env) (t:T.typ) : ML T.reader =
 ///
 /// Other output expressions are translated to setters applied to the base variable and rhs
 
-let translate_action_assignment (lhs:A.out_expr) (rhs:A.expr) : ML T.atomic_action =
+let translate_action_assignment (lhs:A.out_expr) (rhs:A.expr)
+  : ML (T.atomic_action & T.decls) =
   let open A in
   match lhs.out_expr_node.v with
   | OE_star ({out_expr_node={v=OE_id i}}) ->
-    T.Action_assignment i (translate_expr rhs)
+    T.Action_assignment i (translate_expr rhs), []
   | _ ->
-    let fn_name = Target.output_setter_name lhs in
-    let base_var = Target.output_base_var lhs in
+    let t_lhs = translate_out_expr lhs in
+    let fn_name = Target.output_setter_name t_lhs in
+    let base_var = Target.output_base_var t_lhs in
     let v = translate_expr rhs in
-    T.Action_call (Ast.with_dummy_range (Ast.to_ident' fn_name))
-      [(T.Identifier base_var, rhs.A.range); v]
+    let act = T.Action_call (Ast.with_dummy_range (Ast.to_ident' fn_name))
+      [(T.Identifier base_var, rhs.A.range); v] in
+    act, [T.Output_type_expr t_lhs false, output_types_attributes]
 
-let rec translate_action (a:A.action) : ML T.action =
+    // let oe_bt, decls1 = translate_typ (A.out_expr_bt lhs) in
+    // let oe_t, decls2 = translate_typ (A.out_expr_t lhs) in
+
+    // let decls = [
+    //   Target.Output_type_val oe_bt, output_types_attributes;
+    //   Target.Output_type_val oe_t, output_types_attributes;
+    //   Target.Output_type_getter lhs.out_expr_node.v oe_t oe_bt, output_types_attributes] in
+
+    // act, decls
+
+let rec translate_action (a:A.action) : ML (T.action & T.decls) =
   let translate_atomic_action (a:A.atomic_action)
-    : ML T.atomic_action
+    : ML (T.atomic_action & T.decls)
     = match a with
       | Action_return e ->
-        T.Action_return (translate_expr e)
+        T.Action_return (translate_expr e), []
       | Action_abort ->
-        T.Action_abort
+        T.Action_abort, []
       | Action_field_pos ->
-        T.Action_field_pos
+        T.Action_field_pos, []
       | Action_field_ptr ->
-        T.Action_field_ptr
+        T.Action_field_ptr, []
       | Action_deref i ->
-        T.Action_deref i
+        T.Action_deref i, []
       | Action_assignment lhs rhs ->
         translate_action_assignment lhs rhs
       | Action_call f args ->
-        T.Action_call f (List.map translate_expr args)
+        T.Action_call f (List.map translate_expr args), []
   in
   match a.v with
   | Atomic_action a ->
-    T.Atomic_action (translate_atomic_action a)
+    let act, ds = translate_atomic_action a in
+    T.Atomic_action act, ds
 
   | Action_seq hd tl ->
-    T.Action_seq (translate_atomic_action hd) (translate_action tl)
+    let hd, ds1 = translate_atomic_action hd in
+    let tl, ds2 = translate_action tl in
+    T.Action_seq hd tl, ds1@ds2
 
   | Action_ite hd then_ (Some else_) ->
-    T.Action_ite (translate_expr hd) (translate_action then_) (translate_action else_)
+    let then_, ds_then = translate_action then_ in
+    let else_, ds_else = translate_action else_ in
+    T.Action_ite (translate_expr hd) then_ else_, ds_then @ ds_else
 
   | Action_ite hd then_ None ->
+    let then_, ds_then = translate_action then_ in
     T.Action_ite (translate_expr hd)
-                 (translate_action then_)
-                 (T.Atomic_action (T.Action_return (T.mk_expr (T.Constant A.Unit))))
+                 then_
+                 (T.Atomic_action (T.Action_return (T.mk_expr (T.Constant A.Unit)))),
+    ds_then
 
   | Action_let i a k ->
-    T.Action_let i (translate_atomic_action a) (translate_action k)
+    let a, ds1 = translate_atomic_action a in
+    let k, ds2 = translate_action k in
+    T.Action_let i a k, ds1 @ ds2
 
 let rec parser_is_constant_size_without_actions
   (env: global_env)
@@ -755,9 +832,10 @@ let make_zero (r: range) (t: typ) : ML T.expr =
   let it = typ_as_integer_type t in
   (T.Constant (Int it 0), r)
 
-let translate_field (f:A.field) : ML T.struct_field =
+#push-options "--z3rlimit_factor 4"
+let translate_field (f:A.field) : ML (T.struct_field & T.decls) =
     let sf = f.v in
-    let t = translate_typ sf.field_type in
+    let t, ds1 = translate_typ sf.field_type in
     let t =
         let mk_at_most t e : ML T.typ =
           let e = translate_expr e in
@@ -788,13 +866,15 @@ let translate_field (f:A.field) : ML T.struct_field =
       | Some e ->
         T.T_refine t (Some sf.field_ident, translate_expr e)
     in
-    let t =
+    let t, ds2 =
       match sf.field_action with
-      | None -> t
+      | None -> t, []
       | Some (a, false) ->
-        T.T_with_action t (translate_action a)
+        let a, ds2 = translate_action a in
+        T.T_with_action t a, ds2
       | Some (a, _) ->
-        T.T_with_dep_action t (Some sf.field_ident, translate_action a)
+        let a, ds2 = translate_action a in
+        T.T_with_dep_action t (Some sf.field_ident, a), ds2
     in
     let t : T.typ =
       match f.comments with
@@ -811,7 +891,8 @@ let translate_field (f:A.field) : ML T.struct_field =
     else
       T.({sf_dependence=sf.field_dependence;
           sf_ident=sf.field_ident;
-          sf_typ=t})
+          sf_typ=t}), ds1@ds2
+#pop-options
 
 let nondep_group = list T.field
 let grouped_fields = list (either T.field nondep_group)
@@ -1176,10 +1257,10 @@ let translate_switch_case_type (genv:global_env) (tdn:T.typedef_name) (sw:Ast.sw
   let sc = translate_expr sc in
   let env = List.rev tdn.T.td_params in
   let translate_one_case f : ML _ = 
-    let sf = translate_field f in
+    let sf, ds = translate_field f in
     let decls, sfs = hoist_refinements genv tdn [sf] in
     let sf = List.hd sfs in
-    decls, sf
+    ds@decls, sf
   in
   let rest, default_t, decls =
     if List.length cases > 0
@@ -1199,11 +1280,11 @@ let translate_switch_case_type (genv:global_env) (tdn:T.typedef_name) (sw:Ast.sw
       match case with
       | DefaultCase _ -> failwith "Impossible"
       | Case e f ->
-        let open T in
+        //let open T in
         let decls', sf = translate_one_case f in
-        let guard = T.mk_expr (App Eq [sc; translate_expr e]) in
-        let t = T_if_else guard sf.sf_typ t_else in
-        let field_name = Printf.sprintf "%s_ite_%d" (ident_name tdn.td_name) n in
+        let guard = T.mk_expr (T.App T.Eq [sc; translate_expr e]) in
+        let t = T.T_if_else guard sf.T.sf_typ t_else in
+        let field_name = Printf.sprintf "%s_ite_%d" (ident_name tdn.T.td_name) n in
         let td, tdef = hoist_one_type_definition true genv env tdn field_name t in
         tdef, decls@decls'@[td], n + 1)
     rest
@@ -1219,13 +1300,13 @@ let translate_decl (env:global_env) (d:A.decl) : ML (list T.decl) =
     failwith (Printf.sprintf "Untyped definition remains after elaboration: %s" (ident_to_string i))
 
   | Define i (Some t) s ->
-    let t = translate_typ t in
-    [with_comments (T.Definition (i, [], t, T.mk_expr (T.Constant s))) d.d_exported d.d_decl.comments]
+    let t, ds = translate_typ t in
+    ds@[with_comments (T.Definition (i, [], t, T.mk_expr (T.Constant s))) d.d_exported d.d_decl.comments]
 
   | TypeAbbrev t i ->
     let tdn = make_tdn i in
-    let t = translate_typ t in
-    let tdn = translate_typedef_name tdn [] in
+    let t, ds1 = translate_typ t in
+    let tdn, ds2 = translate_typedef_name tdn [] in
     let p = parse_typ env i "" t in
     let open T in
     add_parser_kind_nz env tdn.td_name p.p_kind.pk_nz p.p_kind.pk_weak_kind;
@@ -1238,13 +1319,13 @@ let translate_decl (env:global_env) (d:A.decl) : ML (list T.decl) =
         decl_validator = make_validator env p;
         decl_reader = reader;
     } in
-    [with_comments (Type_decl td) d.d_exported A.(d.d_decl.comments)]
+    ds1@ds2@[with_comments (Type_decl td) d.d_exported A.(d.d_decl.comments)]
 
   | Enum t i ids ->
     let ids = Desugar.check_desugared_enum_cases ids in
     let tdn = make_tdn i in
-    let typ = translate_typ t in
-    let tdn = translate_typedef_name tdn [] in
+    let typ, ds1 = translate_typ t in
+    let tdn, ds2 = translate_typedef_name tdn [] in
     let refined_typ = make_enum_typ typ ids in
     let p = parse_typ env i "" refined_typ in
     let open T in
@@ -1258,11 +1339,14 @@ let translate_decl (env:global_env) (d:A.decl) : ML (list T.decl) =
         decl_validator = make_validator env p;
         decl_reader = reader;
     } in
-    [with_comments (Type_decl td) d.d_exported A.(d.d_decl.comments)]
+    ds1@ds2@[with_comments (Type_decl td) d.d_exported A.(d.d_decl.comments)]
 
   | Record tdn params _ ast_fields ->
-    let tdn = translate_typedef_name tdn params in
-    let fields = List.map translate_field ast_fields in
+    let tdn, ds1 = translate_typedef_name tdn params in
+    let fields, ds2 =
+      List.fold_left (fun (fields, ds) f ->
+        let field, ds' = translate_field f in
+        fields@[field], ds@ds') ([], []) ast_fields in
     let hoists, fields = hoist_refinements env tdn fields in
     let p = parse_fields env tdn fields in
     let open T in
@@ -1277,11 +1361,11 @@ let translate_decl (env:global_env) (d:A.decl) : ML (list T.decl) =
           decl_validator = make_validator env p;
           decl_reader = reader
     } in
-    hoists @ [with_comments (Type_decl td) d.d_exported A.(d.d_decl.comments)]
+   ds1@ds2@hoists @ [with_comments (Type_decl td) d.d_exported A.(d.d_decl.comments)]
 
   | CaseType tdn0 params switch_case ->
-    let tdn = translate_typedef_name tdn0 params in
-    let t, decls = translate_switch_case_type env tdn switch_case in
+    let tdn, ds1 = translate_typedef_name tdn0 params in
+    let t, ds2 = translate_switch_case_type env tdn switch_case in
     let p = parse_typ env tdn0.typedef_name "" t in
     let open T in
     add_parser_kind_nz env tdn.td_name p.p_kind.pk_nz p.p_kind.pk_weak_kind;
@@ -1294,9 +1378,9 @@ let translate_decl (env:global_env) (d:A.decl) : ML (list T.decl) =
           decl_validator = make_validator env p;
         decl_reader = reader;
     } in
-    decls @ [with_comments (Type_decl td) d.d_exported A.(d.d_decl.comments)]
+    ds1 @ ds2 @ [with_comments (Type_decl td) d.d_exported A.(d.d_decl.comments)]
 
-  | OutputType out_t -> [with_comments (T.Output_type out_t) d.d_exported A.(d.d_decl.comments)]
+  | OutputType out_t -> []
 
 noeq
 type translate_env = {
